Update

Gvf_Temporal_Logic.thy
@@ -9,6 +9,7 @@ theory Gvf_Temporal_Logic imports Gvf_Agent_Specification begin
 section \<open>Syntax\<close> 
 
 datatype 'a \<Phi>\<^sub>T =
+  Falsity (\<open>\<bottom>\<^sub>T\<close>) |
   Atom 'a |
   Negation \<open>'a \<Phi>\<^sub>T\<close> (\<open>\<not>\<^sub>T\<close>) | 
   Implication \<open>'a \<Phi>\<^sub>T\<close> \<open>'a \<Phi>\<^sub>T\<close> (infixr \<open>\<longrightarrow>\<^sub>T\<close> 60) | 
@@ -20,8 +21,17 @@ datatype 'a \<Phi>\<^sub>T =
 \<comment> \<open>The type for temporal logic (mental state) formulas including enabledness.\<close>
 type_synonym \<Phi>\<^sub>T\<^sub>E = \<open>Atom\<^sub>E \<Phi>\<^sub>T\<close>
 
+\<comment> \<open>A number of other well known temporal operators can be defined in terms of the operator until.\<close> 
+
+\<comment> \<open>Operator: always\<close>
+definition always :: \<open>'a \<Phi>\<^sub>T \<Rightarrow> 'a \<Phi>\<^sub>T\<close> (\<open>\<box>\<close>) where
+  \<open>\<box>\<phi> \<equiv> \<phi> until \<bottom>\<^sub>T\<close>
+
+definition eventuality :: \<open>'a \<Phi>\<^sub>T \<Rightarrow> 'a \<Phi>\<^sub>T\<close> (\<open>\<diamondop>\<close>) where
+  \<open>\<diamondop>\<phi> \<equiv> \<not>\<^sub>T (\<box> (\<not>\<^sub>T\<phi>))\<close>
+
 \<comment> \<open>Operator: unless\<close>
-abbreviation unless :: \<open>'a \<Phi>\<^sub>T \<Rightarrow> 'a \<Phi>\<^sub>T \<Rightarrow> 'a \<Phi>\<^sub>T\<close> (infix \<open>unless\<close> 55) where
+definition unless :: \<open>'a \<Phi>\<^sub>T \<Rightarrow> 'a \<Phi>\<^sub>T \<Rightarrow> 'a \<Phi>\<^sub>T\<close> (infix \<open>unless\<close> 55) where
   \<open>\<phi> unless \<psi> \<equiv> \<phi> \<longrightarrow>\<^sub>T (\<phi> until \<psi>)\<close>
 
 fun to_\<Phi>\<^sub>T :: \<open>'a \<Phi>\<^sub>P \<Rightarrow> 'a \<Phi>\<^sub>T\<close> (\<open>_\<^sup>T\<close> [100]) where
@@ -31,16 +41,19 @@ fun to_\<Phi>\<^sub>T :: \<open>'a \<Phi>\<^sub>P \<Rightarrow> 'a \<Phi>\<^sub>
   \<open>(p \<^bold>\<or> q)\<^sup>T = (p\<^sup>T \<or>\<^sub>T q\<^sup>T)\<close> |
   \<open>(p \<^bold>\<and> q)\<^sup>T = (p\<^sup>T \<and>\<^sub>T q\<^sup>T)\<close>
 
+section \<open>Semantics\<close>
+
 context single_agent_program begin
 
 fun semantics\<^sub>T :: \<open>trace \<Rightarrow> nat \<Rightarrow> \<Phi>\<^sub>T\<^sub>E \<Rightarrow> bool\<close> (\<open>_, _ \<Turnstile>\<^sub>T\<close> [50]) where
+  \<open>s, i \<Turnstile>\<^sub>T \<bottom>\<^sub>T = False\<close> |
   \<open>s, i \<Turnstile>\<^sub>T (Atom x) = ((\<Phi>\<^sub>P.Atom x)\<^bold>[s i\<^bold>]\<^sub>E)\<close> |
   \<open>s, i \<Turnstile>\<^sub>T (\<not>\<^sub>T p) = (\<not> (s, i \<Turnstile>\<^sub>T p))\<close> |
   \<open>s, i \<Turnstile>\<^sub>T (p \<longrightarrow>\<^sub>T q) = ((s, i \<Turnstile>\<^sub>T p) \<longrightarrow> (s, i \<Turnstile>\<^sub>T q))\<close> |
   \<open>s, i \<Turnstile>\<^sub>T (p \<or>\<^sub>T q) = ((s, i \<Turnstile>\<^sub>T p) \<or> (s, i \<Turnstile>\<^sub>T q))\<close> |
   \<open>s, i \<Turnstile>\<^sub>T (p \<and>\<^sub>T q) = ((s, i \<Turnstile>\<^sub>T p) \<and> (s, i \<Turnstile>\<^sub>T q))\<close> |
   \<open>s, i \<Turnstile>\<^sub>T init = (i = 0)\<close> |
-  \<open>s, i \<Turnstile>\<^sub>T (\<phi> until \<psi>) = ((\<exists> j \<ge> i. (s, j \<Turnstile>\<^sub>T \<psi>) \<and> (\<forall>k \<ge> i. j > k \<longrightarrow> (s, k \<Turnstile>\<^sub>T \<phi>))) \<or> (\<forall>k \<ge> i. (s, k \<Turnstile>\<^sub>T \<phi>)))\<close>
+  \<open>s, i \<Turnstile>\<^sub>T (\<phi> until \<psi>) = ((\<exists> j \<ge> i. s, j \<Turnstile>\<^sub>T \<psi> \<and> (\<forall>k \<ge> i. j > k \<longrightarrow> s, k \<Turnstile>\<^sub>T \<phi>)) \<or> (\<forall>k \<ge> i. s, k \<Turnstile>\<^sub>T \<phi>))\<close>
 
 lemma sem\<^sub>T\<^sub>E_equiv: \<open>(\<forall>M. semantics\<^sub>E M p) \<longleftrightarrow> (\<forall>s i. (p\<^bold>[s i\<^bold>]\<^sub>E))\<close> 
   using st_nth.simps(1) by metis
@@ -53,11 +66,93 @@ lemma \<open>(\<forall>M. semantics\<^sub>E M p) \<longleftrightarrow> (\<forall
 abbreviation semantics_trace\<^sub>T\<^sub>E :: \<open>trace set \<Rightarrow> \<Phi>\<^sub>T\<^sub>E \<Rightarrow> bool\<close> (infix \<open>\<Turnstile>\<^sub>T#\<close> 50) where
   \<open>S \<Turnstile>\<^sub>T# \<phi> \<equiv> \<forall>s\<in>S. \<forall>i. (s, i \<Turnstile>\<^sub>T \<phi>)\<close>
 
+section \<open>Relations between Hoare Logic and Temporal Logic\<close>
+
+subsection \<open>Unless\<close>
+
 \<comment> \<open>Theorem 4.15\<close>
 theorem unless_ht: \<open>(\<forall>b \<in> \<Pi>. (\<Turnstile>\<^sub>H \<^bold>{ \<phi> \<^bold>\<and> \<^bold>\<not> \<psi> \<^bold>} ((fst b) \<triangleright> do (snd b)) \<^bold>{ \<phi> \<^bold>\<or> \<psi> \<^bold>})) \<longleftrightarrow> Agent \<Turnstile>\<^sub>T# \<phi>\<^sup>E\<^sup>T unless \<psi>\<^sup>E\<^sup>T\<close>
 proof
-  assume \<open>\<forall>b \<in> \<Pi>. (\<Turnstile>\<^sub>H \<^bold>{ \<phi> \<^bold>\<and> \<^bold>\<not> \<psi> \<^bold>} ((fst b) \<triangleright> do (snd b)) \<^bold>{ \<phi> \<^bold>\<or> \<psi> \<^bold>})\<close>
-  show \<open>Agent \<Turnstile>\<^sub>T# \<phi>\<^sup>E\<^sup>T unless \<psi>\<^sup>E\<^sup>T\<close> sorry
+  assume *: \<open>\<forall>b \<in> \<Pi>. (\<Turnstile>\<^sub>H \<^bold>{ \<phi> \<^bold>\<and> \<^bold>\<not> \<psi> \<^bold>} ((fst b) \<triangleright> do (snd b)) \<^bold>{ \<phi> \<^bold>\<or> \<psi> \<^bold>})\<close>
+  show \<open>Agent \<Turnstile>\<^sub>T# \<phi>\<^sup>E\<^sup>T unless \<psi>\<^sup>E\<^sup>T\<close> (is \<open>Agent \<Turnstile>\<^sub>T# ?\<phi> unless ?\<psi>\<close>)
+  proof (rule ccontr)
+    assume \<open>\<not> Agent \<Turnstile>\<^sub>T# ?\<phi> unless ?\<psi>\<close>
+    then obtain s i where \<open>\<not> (s, i \<Turnstile>\<^sub>T (?\<phi> unless ?\<psi>))\<close> \<open>s \<in> Agent\<close> by auto
+    then have \<open>s, i \<Turnstile>\<^sub>T ?\<phi>\<close> \<open>\<not> (s, i \<Turnstile>\<^sub>T (?\<phi> until ?\<psi>))\<close> unfolding unless_def by simp_all
+    then have \<open>\<not>(\<exists> j \<ge> i. s, j \<Turnstile>\<^sub>T ?\<psi>) \<and> (\<exists>k \<ge> i. s, k \<Turnstile>\<^sub>T (\<not>\<^sub>T ?\<phi>)) \<or> (\<exists> j > i. s, j \<Turnstile>\<^sub>T ?\<psi>) \<and> (\<forall> j > i. s, j \<Turnstile>\<^sub>T ?\<psi> \<longrightarrow> \<not>(\<forall>k \<ge> i. j > k \<longrightarrow> s, k \<Turnstile>\<^sub>T ?\<phi>))\<close> by auto
+    then show False 
+    proof
+      assume a: \<open>\<not> (\<exists>j\<ge>i. s, j \<Turnstile>\<^sub>T ?\<psi>) \<and> (\<exists>k\<ge>i. s, k \<Turnstile>\<^sub>T (\<not>\<^sub>T ?\<phi>))\<close>
+      let ?P = \<open>\<lambda>x. x \<ge> i \<and> s, x \<Turnstile>\<^sub>T (\<not>\<^sub>T ?\<phi>)\<close>
+      have \<open>\<not> ?P 0\<close> using \<open>s, i \<Turnstile>\<^sub>T ?\<phi>\<close> by fastforce
+      moreover obtain n where \<open>?P n\<close> using a by auto
+      ultimately have \<open>\<exists>k\<le>n. (\<forall>i<k. \<not> ?P i) \<and> ?P k\<close> using ex_least_nat_le[where P=\<open>?P\<close>] by simp
+      then obtain k where Pk: \<open>k \<le> n \<and> (\<forall>i<k. \<not> ?P i) \<and> ?P k\<close> by auto
+      moreover from this have \<open>k > i\<close> using \<open>s, i \<Turnstile>\<^sub>T ?\<phi>\<close> by fastforce
+      ultimately have \<open>\<not> ?P (k - 1)\<close> by simp
+      with \<open>k > i\<close> have \<open>s, k - 1 \<Turnstile>\<^sub>T (?\<phi> \<and>\<^sub>T \<not>\<^sub>T ?\<psi>)\<close> using a by simp
+      then have \<open>st_nth s (k - 1) \<Turnstile>\<^sub>M \<phi> \<^bold>\<and> \<^bold>\<not> \<psi>\<close> by (simp add: sem\<^sub>T\<^sub>E_equiv2 transfer_semantics\<^sub>M)
+      moreover have \<open>?P k\<close> using Pk by simp
+      then have \<open>s, k \<Turnstile>\<^sub>T (\<not>\<^sub>T ?\<phi> \<and>\<^sub>T \<not>\<^sub>T ?\<psi>)\<close> using a \<open>k > i\<close> by simp
+      then have \<open>st_nth s k \<Turnstile>\<^sub>M \<^bold>\<not> \<phi> \<^bold>\<and> \<^bold>\<not> \<psi>\<close> by (simp add: sem\<^sub>T\<^sub>E_equiv2 transfer_semantics\<^sub>M)
+      moreover obtain b where \<open>(fst b, snd b) = act_nth s (k - 1)\<close> by simp
+      moreover from this have \<open>b \<in> \<Pi>\<close> using \<open>s \<in> Agent\<close> trace_in_\<Pi> unfolding Agent_def by simp
+      with * have \<open>\<forall> s \<in> Agent. \<forall>i. ((\<phi> \<^bold>\<and> \<^bold>\<not> \<psi>)\<^bold>[s i\<^bold>]\<^sub>M) \<and> ((fst b) \<triangleright> do (snd b)) = (act_nth s i) \<longrightarrow> ((\<phi> \<^bold>\<or> \<psi>)\<^bold>[s (i+1)\<^bold>]\<^sub>M)\<close>
+        using semantics\<^sub>H.simps(2) by blast
+      then have \<open>((\<phi> \<^bold>\<and> \<^bold>\<not> \<psi>)\<^bold>[s (k-1)\<^bold>]\<^sub>M) \<and> ((fst b) \<triangleright> do (snd b)) = (act_nth s (k-1)) \<longrightarrow> ((\<phi> \<^bold>\<or> \<psi>)\<^bold>[s ((k-1)+1)\<^bold>]\<^sub>M)\<close> 
+        using \<open>s \<in> Agent\<close> by simp
+      with \<open>k > i\<close> have \<open>((\<phi> \<^bold>\<and> \<^bold>\<not> \<psi>)\<^bold>[s (k-1)\<^bold>]\<^sub>M) \<and> ((fst b) \<triangleright> do (snd b)) = (act_nth s (k-1)) \<longrightarrow> ((\<phi> \<^bold>\<or> \<psi>)\<^bold>[s k\<^bold>]\<^sub>M)\<close> 
+        by simp
+      ultimately show False by simp
+    next
+      assume a: \<open>(\<exists> j > i. s, j \<Turnstile>\<^sub>T ?\<psi>) \<and> (\<forall> j > i. s, j \<Turnstile>\<^sub>T ?\<psi> \<longrightarrow> \<not>(\<forall>k \<ge> i. j > k \<longrightarrow> s, k \<Turnstile>\<^sub>T ?\<phi>))\<close>
+      let ?P = \<open>\<lambda>x. x > i \<and> s, x \<Turnstile>\<^sub>T ?\<psi>\<close>
+      have \<open>\<not> ?P 0\<close> by simp
+      moreover obtain n where \<open>?P n\<close> using a by auto
+      ultimately have \<open>\<exists>k\<le>n. (\<forall>i<k. \<not> ?P i) \<and> ?P k\<close> using ex_least_nat_le[where P=\<open>?P\<close>] by simp
+      then obtain k where Pk: \<open>k \<le> n \<and> (\<forall>i<k. \<not> ?P i) \<and> ?P k\<close> by auto
+      let ?P' = \<open>\<lambda>x. i < x \<and> x < k \<and> \<not> s, x \<Turnstile>\<^sub>T ?\<phi>\<close>
+      have \<open>\<not> ?P' 0\<close> by simp
+      moreover obtain n' where \<open>?P' n'\<close> using Pk \<open>s, i \<Turnstile>\<^sub>T ?\<phi>\<close> le_neq_trans a by blast
+      ultimately have \<open>\<exists>j\<le>n'. (\<forall>i<j. \<not> ?P' i) \<and> ?P' j\<close> using ex_least_nat_le[where P=\<open>?P'\<close>] by simp
+      then obtain j where Pj: \<open>j \<le> n' \<and> (\<forall>i<j. \<not> ?P' i) \<and> ?P' j\<close> by auto
+      then have \<open>\<not> ?P' (j - 1)\<close> by simp
+      moreover have \<open>j - 1 < k\<close> using Pj by auto
+      ultimately have \<open>s, j - 1 \<Turnstile>\<^sub>T ?\<phi>\<close> 
+      proof (cases \<open>i < j - 1\<close>)
+        case False
+        then have \<open>i = j - 1\<close> using Pj by auto
+        with \<open>s, i \<Turnstile>\<^sub>T ?\<phi>\<close> show ?thesis by simp
+      qed simp
+      moreover have \<open>\<not> ?P (j - 1)\<close> using Pk \<open>j - 1 < k\<close> by blast
+      then have \<open>s, j - 1 \<Turnstile>\<^sub>T (\<not>\<^sub>T ?\<psi>)\<close>
+      proof (cases \<open>i < j - 1\<close>)
+        case False
+        then have \<open>i = j - 1\<close> using Pj by auto
+        with \<open>\<not> s, i \<Turnstile>\<^sub>T (?\<phi> until ?\<psi>)\<close> show ?thesis by fastforce
+      qed simp
+      ultimately have \<open>s, j - 1 \<Turnstile>\<^sub>T (?\<phi> \<and>\<^sub>T \<not>\<^sub>T ?\<psi>)\<close> by simp
+      then have \<open>st_nth s (j - 1) \<Turnstile>\<^sub>M \<phi> \<^bold>\<and> \<^bold>\<not> \<psi>\<close> by (simp add: sem\<^sub>T\<^sub>E_equiv2 transfer_semantics\<^sub>M)
+      moreover 
+      {
+        have \<open>\<not> s, j \<Turnstile>\<^sub>T ?\<phi>\<close> using Pj by simp
+        moreover have \<open>j < k\<close> using Pj by simp
+        then have \<open>\<not> ?P j\<close> using Pk by simp
+        then have \<open>\<not> s, j \<Turnstile>\<^sub>T ?\<psi>\<close> using Pj by simp
+        ultimately have \<open>s, j \<Turnstile>\<^sub>T (\<not>\<^sub>T ?\<phi> \<and>\<^sub>T \<not>\<^sub>T ?\<psi>)\<close> by simp
+        then have \<open>st_nth s j \<Turnstile>\<^sub>M \<^bold>\<not> \<phi> \<^bold>\<and> \<^bold>\<not> \<psi>\<close> by (simp add: sem\<^sub>T\<^sub>E_equiv2 transfer_semantics\<^sub>M)
+      }
+      moreover obtain b where \<open>(fst b, snd b) = act_nth s (j - 1)\<close> by simp
+      moreover from this have \<open>b \<in> \<Pi>\<close> using \<open>s \<in> Agent\<close> trace_in_\<Pi> unfolding Agent_def by simp
+      with * have \<open>\<forall> s \<in> Agent. \<forall>i. ((\<phi> \<^bold>\<and> \<^bold>\<not> \<psi>)\<^bold>[s i\<^bold>]\<^sub>M) \<and> ((fst b) \<triangleright> do (snd b)) = (act_nth s i) \<longrightarrow> ((\<phi> \<^bold>\<or> \<psi>)\<^bold>[s (i+1)\<^bold>]\<^sub>M)\<close>
+        using semantics\<^sub>H.simps(2) by blast
+      then have \<open>((\<phi> \<^bold>\<and> \<^bold>\<not> \<psi>)\<^bold>[s (j-1)\<^bold>]\<^sub>M) \<and> ((fst b) \<triangleright> do (snd b)) = (act_nth s (j-1)) \<longrightarrow> ((\<phi> \<^bold>\<or> \<psi>)\<^bold>[s ((j-1)+1)\<^bold>]\<^sub>M)\<close> 
+        using \<open>s \<in> Agent\<close> by simp
+      with Pj have \<open>((\<phi> \<^bold>\<and> \<^bold>\<not> \<psi>)\<^bold>[s (j-1)\<^bold>]\<^sub>M) \<and> ((fst b) \<triangleright> do (snd b)) = (act_nth s (j-1)) \<longrightarrow> ((\<phi> \<^bold>\<or> \<psi>)\<^bold>[s j\<^bold>]\<^sub>M)\<close> 
+        by simp
+      ultimately show False by simp
+    qed
+  qed
 next
   assume \<open>Agent \<Turnstile>\<^sub>T# \<phi>\<^sup>E\<^sup>T unless \<psi>\<^sup>E\<^sup>T\<close> (is \<open>Agent \<Turnstile>\<^sub>T# ?\<phi> unless ?\<psi>\<close>)
   show \<open>\<forall>b \<in> \<Pi>. (\<Turnstile>\<^sub>H \<^bold>{ \<phi> \<^bold>\<and> \<^bold>\<not> \<psi> \<^bold>} ((fst b) \<triangleright> do (snd b)) \<^bold>{ \<phi> \<^bold>\<or> \<psi> \<^bold>})\<close>
@@ -77,17 +172,27 @@ next
           proof (cases \<open>st_nth s i \<Turnstile>\<^sub>M \<phi>\<close>)
             case True
             then have \<open>s, i \<Turnstile>\<^sub>T ?\<phi>\<close> by (simp add: sem\<^sub>T\<^sub>E_equiv2 transfer_semantics\<^sub>M)
-            with \<open>Agent \<Turnstile>\<^sub>T# ?\<phi> unless ?\<psi>\<close> have \<open>s, i \<Turnstile>\<^sub>T (?\<phi> until ?\<psi>)\<close> using \<open>s \<in> Agent\<close> by simp
+            with \<open>Agent \<Turnstile>\<^sub>T# ?\<phi> unless ?\<psi>\<close> have \<open>s, i \<Turnstile>\<^sub>T (?\<phi> until ?\<psi>)\<close> using \<open>s \<in> Agent\<close> unfolding unless_def by simp
+            then have \<open>(\<exists> j \<ge> i. (s, j \<Turnstile>\<^sub>T ?\<psi>) \<and> (\<forall>k \<ge> i. j > k \<longrightarrow> (s, k \<Turnstile>\<^sub>T ?\<phi>))) \<or> (\<forall>k \<ge> i. (s, k \<Turnstile>\<^sub>T ?\<phi>))\<close> by simp
+            then obtain j where *: \<open>(j \<ge> i \<and> s, j \<Turnstile>\<^sub>T ?\<psi> \<and> (\<forall>k \<ge> i. j > k \<longrightarrow> s, k \<Turnstile>\<^sub>T ?\<phi>)) \<or> s, i + 1 \<Turnstile>\<^sub>T ?\<phi>\<close> by auto
             then show ?thesis
-            proof (cases \<open>st_nth s i \<Turnstile>\<^sub>M \<psi>\<close>)
+            proof (cases \<open>j > i + 1\<close>)
+              case True
+              with * have \<open>s, (i + 1) \<Turnstile>\<^sub>T ?\<phi>\<close> by auto
+              then have \<open>st_nth s (i + 1) \<Turnstile>\<^sub>M \<phi> \<^bold>\<or> \<psi>\<close> by (simp add: sem\<^sub>T\<^sub>E_equiv2 transfer_semantics\<^sub>M)
+              then show ?thesis by simp
+            next
               case False
-              show ?thesis
-              proof
-                assume \<open>st_nth s i \<Turnstile>\<^sub>M \<phi> \<^bold>\<and> \<^bold>\<not> \<psi> \<and> (fst b, snd b) = act_nth s i\<close>
-                then have \<open>(fst b, snd b) = act_nth s i\<close> by simp
-                show \<open>st_nth s (i + 1) \<Turnstile>\<^sub>M \<phi> \<^bold>\<or> \<psi>\<close> sorry
-              qed
-            qed simp
+              with * have **: \<open>s, i \<Turnstile>\<^sub>T ?\<psi> \<or> s, i + 1 \<Turnstile>\<^sub>T ?\<psi> \<or> s, i + 1 \<Turnstile>\<^sub>T ?\<phi>\<close>
+                by (metis discrete order.not_eq_order_implies_strict)
+              then show ?thesis
+              proof (cases \<open>st_nth s i \<Turnstile>\<^sub>M \<psi>\<close>)
+                case False
+                then have \<open>\<not> s, i \<Turnstile>\<^sub>T ?\<psi>\<close> by (simp add: sem\<^sub>T\<^sub>E_equiv2 transfer_semantics\<^sub>M)
+                with ** have \<open>s, i + 1 \<Turnstile>\<^sub>T ?\<psi> \<or> s, i + 1 \<Turnstile>\<^sub>T ?\<phi>\<close> by simp
+                then show ?thesis using sem\<^sub>T\<^sub>E_equiv2 transfer_semantics\<^sub>M by auto
+              qed simp
+            qed
           qed simp
         qed
       qed
@@ -95,6 +200,56 @@ next
     qed
   qed
 qed
+
+subsection \<open>Ensures\<close>
+
+definition ensures :: \<open>'a \<Phi>\<^sub>T \<Rightarrow> 'a \<Phi>\<^sub>T \<Rightarrow> 'a \<Phi>\<^sub>T\<close> (infix \<open>ensures\<close> 55) where
+  \<open>\<phi> ensures \<psi> \<equiv> (\<phi> unless \<psi>) \<and>\<^sub>T (\<phi> \<longrightarrow>\<^sub>T \<diamondop>\<psi>)\<close>
+
+\<comment> \<open>Theorem 4.16\<close>
+theorem ex_ensures:
+  assumes \<open>\<forall>b \<in> \<Pi>. (\<Turnstile>\<^sub>H \<^bold>{ \<phi> \<^bold>\<and> \<^bold>\<not> \<psi> \<^bold>} ((fst b) \<triangleright> do (snd b)) \<^bold>{ \<phi> \<^bold>\<or> \<psi> \<^bold>})\<close> 
+      and \<open>\<exists>b \<in> \<Pi>. (\<Turnstile>\<^sub>H \<^bold>{ \<phi> \<^bold>\<and> \<^bold>\<not> \<psi> \<^bold>} ((fst b) \<triangleright> do (snd b)) \<^bold>{ \<psi> \<^bold>})\<close>
+    shows \<open>Agent \<Turnstile>\<^sub>T# \<phi>\<^sup>E\<^sup>T ensures \<psi>\<^sup>E\<^sup>T\<close> (is \<open>Agent \<Turnstile>\<^sub>T# ?\<phi> ensures ?\<psi>\<close>)
+proof
+  fix s
+  assume \<open>s \<in> Agent\<close>
+  show \<open>\<forall>i. s, i \<Turnstile>\<^sub>T (?\<phi> ensures ?\<psi>)\<close>
+  proof 
+    fix i
+    have \<open>\<forall>i. s, i \<Turnstile>\<^sub>T (?\<phi> unless ?\<psi>)\<close> using assms(1) \<open>s \<in> Agent\<close> unless_ht by simp
+    moreover have \<open>s, i \<Turnstile>\<^sub>T (?\<phi> \<longrightarrow>\<^sub>T \<diamondop> ?\<psi>)\<close>
+    proof -
+      have \<open>fair_trace s\<close> using \<open>s \<in> Agent\<close> unfolding Agent_def by simp
+      show ?thesis   
+      proof (rule ccontr)
+        assume negev: \<open>\<not> s, i \<Turnstile>\<^sub>T (?\<phi> \<longrightarrow>\<^sub>T \<diamondop> ?\<psi>)\<close>
+        then have \<open>s, i \<Turnstile>\<^sub>T (?\<phi> \<and>\<^sub>T \<not>\<^sub>T ?\<psi>) \<and> (\<forall>j > i. s, j \<Turnstile>\<^sub>T (\<not>\<^sub>T ?\<psi>))\<close> 
+          unfolding eventuality_def always_def by simp
+        with negev \<open>\<forall>i. s, i \<Turnstile>\<^sub>T (?\<phi> unless ?\<psi>)\<close> have \<open>\<forall>j > i. s, j \<Turnstile>\<^sub>T (?\<phi> \<and>\<^sub>T \<not>\<^sub>T ?\<psi>)\<close> 
+          unfolding unless_def always_def eventuality_def by auto
+        moreover 
+        {
+          from assms(2) obtain b where \<open>b \<in> \<Pi> \<and> (\<forall>i. ((\<phi> \<^bold>\<and> \<^bold>\<not> \<psi>)\<^bold>[s i\<^bold>]\<^sub>M) \<and> ((fst b) \<triangleright> do (snd b)) = (act_nth s i) \<longrightarrow> (\<psi>\<^bold>[s (i+1)\<^bold>]\<^sub>M))\<close> 
+            using \<open>s \<in> Agent\<close> by fastforce
+          then have \<open>b \<in> \<Pi> \<and> (\<forall>j > i. ((\<phi> \<^bold>\<and> \<^bold>\<not> \<psi>)\<^bold>[s j\<^bold>]\<^sub>M) \<and> ((fst b) \<triangleright> do (snd b)) = (act_nth s j) \<longrightarrow> (\<psi>\<^bold>[s (j+1)\<^bold>]\<^sub>M))\<close> 
+            by auto
+          moreover from this have \<open>\<exists>j > i. ((fst b) \<triangleright> do (snd b)) = (act_nth s j)\<close> 
+            using \<open>fair_trace s\<close> unfolding fair_trace_def by fastforce
+          ultimately have \<open>\<exists>j > i. ((\<phi> \<^bold>\<and> \<^bold>\<not> \<psi>)\<^bold>[s j\<^bold>]\<^sub>M) \<longrightarrow> (\<psi>\<^bold>[s (j+1)\<^bold>]\<^sub>M)\<close> by auto
+          moreover from \<open>\<forall>j > i. s, j \<Turnstile>\<^sub>T (?\<phi> \<and>\<^sub>T \<not>\<^sub>T ?\<psi>)\<close> have \<open>\<forall>j > i. ((\<phi> \<^bold>\<and> \<^bold>\<not> \<psi>)\<^bold>[s j\<^bold>]\<^sub>M)\<close> 
+            using sem\<^sub>T\<^sub>E_equiv2 transfer_semantics\<^sub>M by simp
+          ultimately have \<open>\<exists>j > i. (\<psi>\<^bold>[s (j+1)\<^bold>]\<^sub>M)\<close> by auto
+        }
+      ultimately show False using sem\<^sub>T\<^sub>E_equiv2 transfer_semantics\<^sub>M by auto
+      qed
+    qed
+    ultimately show \<open>s, i \<Turnstile>\<^sub>T (?\<phi> ensures ?\<psi>)\<close> by (simp add: ensures_def)
+  qed
+qed
+
+subsection \<open>Leads to operator\<close>
+
 
 end
 end
